theories/DSub/adequacy.v
@@ -4,24 +4,22 @@ From D.DSub Require Import unary_lr.
 
 Import dlang_adequacy.
 
-Theorem adequacy Σ `{HdlangG: dlangPreG Σ} `{!SwapProp (iPropSI Σ)} e e' thp σ σ' T ρ:
-  (forall `{dlangG Σ} `{SwapProp (iPropSI Σ)}, True ⊢ ⟦ T ⟧ₑ ρ e) →
-  rtc erased_step ([e], σ) (thp, σ') → e' ∈ thp →
-  is_Some (to_val e') ∨ reducible e' σ'.
+Theorem adequacy Σ `{HdlangG: dlangPreG Σ} `{SwapProp (iPropSI Σ)} e T:
+  (∀ `(dlangG Σ) `(!SwapProp (iPropSI Σ)), [] ⊨ e : T) →
+  safe e.
 Proof.
-  intros Hlog.
-  eapply (adequacy _) => Hdlang Hswap.
-  iDestruct (Hlog with "[#]") as "H"; iIntros; by [].
+  intros Hlog ?*. eapply (adequacy _).
+  iIntros (??) "Hs". iDestruct Hlog as "#Htyp".
+  by iSpecialize ("Htyp" $! ids with "[#//]"); rewrite hsubst_id.
 Qed.
 
 (* Instead of still assuming semantic typing, here we should assume syntactic
    typing and use the fundamental lemma. But otherwise this follows the general
    instantiation pattern, from e.g.
    https://gitlab.mpi-sws.org/iris/examples/blob/a89dc12821b63eeb9b831d21629ac55ebd601f38/theories/logrel/F_mu_ref/soundness.v#L29-39. *)
-Corollary almost_type_soundness e e' thp σ σ' T:
-  (forall `{dlangG Σ} `{SwapProp (iPropSI Σ)}, True ⊢ ⟦ T ⟧ₑ ids e) →
-  rtc erased_step ([e], σ) (thp, σ') → e' ∈ thp →
-  is_Some (to_val e') ∨ reducible e' σ'.
+Corollary almost_type_soundness e T:
+  (∀ `(dlangG Σ) `(!SwapProp (iPropSI Σ)), [] ⊨ e : T) →
+  safe e.
 Proof.
   intros; eapply (adequacy dlangΣ) => //.
   exact: H.
